src/Examples/ECC/CondSwap.v
@@ -16,13 +16,15 @@ Section Compile.
     forall (locals: Semantics.locals) (mem: Semantics.mem)
            (locals_ok : Semantics.locals -> Prop)
       tr R R' functions T (pred: T -> _ -> Prop)
-      {data} (x y : data) swap x_var x_ptr y_var y_ptr k k_impl
-      (Data : word -> data -> Semantics.mem -> Prop) var,
+      {data} (x y : data) swap swap_var x_var x_ptr y_var y_ptr k k_impl
+      (Data : word -> data -> Semantics.mem -> Prop) tmp,
       x_var <> y_var ->
-      x_var <> var ->
-      var <> y_var ->
+      map.get locals swap_var = Some (word.of_Z (Z.b2z swap)) ->
       map.get locals x_var = Some x_ptr ->
       map.get locals y_var = Some y_ptr ->
+      (* tmp is a strictly temporary variable, confined to one part of the
+         if-clause; it gets unset after use *)
+      map.get locals tmp = None ->
       (Data x_ptr x * Data y_ptr y * R')%sep mem ->
       let v := cswap swap x y in
       (let head := v in
@@ -30,24 +32,55 @@ Section Compile.
         implementing (pred (k head))
         and-locals-post locals_ok
         with-locals
-               (map.put (map.put (map.put locals var x_ptr) x_var y_ptr)
-                        y_var x_ptr)
+               (map.put (map.put locals
+                                 x_var (fst (cswap swap x_ptr y_ptr)))
+                        y_var (snd (cswap swap x_ptr y_ptr)))
         and-memory mem and-trace tr and-rest R
         and-functions functions)) ->
       (let head := v in
        find (cmd.seq
-               (cmd.seq
+               (cmd.cond
+                  (expr.var swap_var)
                   (cmd.seq
-                     (cmd.set var (expr.var x_var))
-                     (cmd.set x_var (expr.var y_var)))
-                  (cmd.set y_var (expr.var var)))
+                     (cmd.seq
+                        (cmd.seq
+                           (cmd.set tmp (expr.var x_var))
+                           (cmd.set x_var (expr.var y_var)))
+                        (cmd.set y_var (expr.var tmp)))
+                     (cmd.unset tmp))
+                  (cmd.skip))
                k_impl)
        implementing (pred (dlet head k))
        and-locals-post locals_ok
        with-locals locals and-memory mem and-trace tr and-rest R
        and-functions functions).
   Proof.
-    repeat straightline'. subst_lets_in_goal. eauto.
+    repeat straightline'.
+    destr (tmp =? x_var); [ congruence | ].
+    destr (tmp =? y_var); [ congruence | ].
+    destruct swap; cbn [Z.b2z cswap fst snd] in *;
+      split_if ltac:(repeat straightline');
+    try (subst_lets_in_goal;
+         rewrite ?word.unsigned_of_Z_0, ?word.unsigned_of_Z_1;
+         congruence); [ | ].
+    { repeat straightline'.
+      match goal with
+      | H : WeakestPrecondition.cmd _ _ _ _ ?l1 _
+        |- WeakestPrecondition.cmd _ _ _ _ ?l2 _ =>
+        replace l2 with l1; [ exact H | apply map.map_ext ]
+      end.
+      subst_lets_in_goal. intros.
+      rewrite !map.get_remove_dec, !map.get_put_dec.
+      repeat destruct_one_match; congruence. }
+    { repeat straightline'.
+      match goal with
+      | H : WeakestPrecondition.cmd _ _ _ _ ?l1 _
+        |- WeakestPrecondition.cmd _ _ _ _ ?l2 _ =>
+        replace l2 with l1; [ exact H | apply map.map_ext ]
+      end.
+      subst_lets_in_goal. intros.
+      rewrite !map.get_put_dec.
+      repeat destruct_one_match; congruence. }
   Qed.
 
   Lemma compile_cswap_pair :
