src/Examples/ECC/Point.v
@@ -16,13 +16,13 @@ Section Compile.
            (locals_ok : Semantics.locals -> Prop)
       tr R functions T (pred: T -> _ -> Prop)
       (x y : Z) (X Y : bignum) k k_impl,
-      eval X = x ->
-      eval Y = y ->
-      let v := (x, y) in
+      (eval X mod M = x mod M)%Z ->
+      (eval Y mod M = y mod M)%Z ->
+      let v := (x mod M, y mod M)%Z in
       (let head := v in
        find k_impl
-       implementing (pred (dlet (eval X)
-                                (fun x => dlet (eval Y)
+       implementing (pred (dlet (eval X mod M)%Z
+                                (fun x => dlet (eval Y mod M)%Z
                                                (fun y => k (x, y)))))
        and-locals-post locals_ok
        with-locals locals and-memory mem and-trace tr and-rest R
@@ -34,6 +34,11 @@ Section Compile.
        with-locals locals and-memory mem and-trace tr and-rest R
        and-functions functions).
   Proof.
-    repeat straightline'. subst; auto.
+    repeat straightline'.
+    repeat match goal with
+             H : (?x mod M = _ mod M)%Z |- _ =>
+             rewrite H in *
+           end.
+    eauto.
   Qed.
 End Compile.
