src/Examples/KVStore/KVStore.v
@@ -1,37 +1,5 @@
 Require Import Rupicola.Lib.Api.
 
-(* TODO: should move upstream to coqutil *)
-Module map.
-  Section __.
-    Context {key value} {map : map.map key value}
-            {map_ok : map.ok map}
-            {key_eqb}
-            {key_eq_dec :
-               forall x y : key, BoolSpec (x = y) (x <> y) (key_eqb x y)}.
-
-    Lemma put_put_diff_comm k1 k2 v1 v2 m :
-      k1 <> k2 ->
-      map.put (map.put m k1 v1) k2 v2 = map.put (map.put m k2 v2) k1 v1.
-    Proof.
-      intros. apply map.map_ext. intros.
-      rewrite !map.get_put_dec;
-        repeat match goal with |- context [key_eqb ?x ?y] =>
-                               destr (key_eqb x y) end;
-        congruence.
-    Qed.
-
-    Lemma put_noop k v m :
-      map.get m k = Some v -> map.put m k v = m.
-    Proof.
-      intros. apply map.map_ext. intros.
-      rewrite !map.get_put_dec;
-        repeat match goal with |- context [key_eqb ?x ?y] =>
-                               destr (key_eqb x y) end;
-        congruence.
-    Qed.
-  End __.
-End map.
-
 Section KVStore.
   Context {semantics : Semantics.parameters}
           {semantics_ok : Semantics.parameters_ok semantics}.
