src/Lib/Core.v
@@ -40,3 +40,36 @@ Coercion name_of_func (f : bedrock_func) := fst f.
 
 Hint Rewrite @map.get_put_diff @map.get_put_same @map.put_put_same
      using (typeclasses eauto || congruence) : mapsimpl.
+
+
+(* TODO: should move upstream to coqutil *)
+Module map.
+  Section __.
+    Context {key value} {map : map.map key value}
+            {map_ok : map.ok map}
+            {key_eqb}
+            {key_eq_dec :
+               forall x y : key, BoolSpec (x = y) (x <> y) (key_eqb x y)}.
+
+    Lemma put_put_diff_comm k1 k2 v1 v2 m :
+      k1 <> k2 ->
+      map.put (map.put m k1 v1) k2 v2 = map.put (map.put m k2 v2) k1 v1.
+    Proof.
+      intros. apply map.map_ext. intros.
+      rewrite !map.get_put_dec;
+        repeat match goal with |- context [key_eqb ?x ?y] =>
+                               destr (key_eqb x y) end;
+        congruence.
+    Qed.
+
+    Lemma put_noop k v m :
+      map.get m k = Some v -> map.put m k v = m.
+    Proof.
+      intros. apply map.map_ext. intros.
+      rewrite !map.get_put_dec;
+        repeat match goal with |- context [key_eqb ?x ?y] =>
+                               destr (key_eqb x y) end;
+        congruence.
+    Qed.
+  End __.
+End map.
